Trace: redefine using new AMMSets

Trace.lean
@@ -4,12 +4,48 @@ import «Tokens»
 import «Swap»
 
 inductive Trace (c: Config): State → Type where
-  | empty (accs: AccountSet): 
+  | empty (accs: AccountSet) 
+    (h: ∀(a: Account) (m: MintedTok), accs a m = 0): 
       Trace c ⟨accs, AMMSet.empty⟩
 
-  | dep0 (rs: Trace c s) (d: Deposit0.Valid s): 
+  | dep0 (s: State) (rs: Trace c s) (d: Deposit0.Valid s): 
       Trace c (Deposit0.apply d)
 
-  | swap (rs: Trace c s) (sw: Swap.Valid c s):
+  | swap (s: State) (rs: Trace c s) (sw: Swap.Valid c s):
       Trace c (Swap.apply sw)
 
+/-
+Proof that 
+m ∈ (Trace c s).state.amms.map.supp → supply m > 0
+
+by induction
+empty (base case): hypothesis is a contradiction
+dep0: trivial
+swap: use IH. 
+      swaps don't change minted token supplies
+-/
+theorem AMMimpSupply 
+(t: Trace c s) (t0 t1: AtomicTok) (h: s.amms.f t0 t1 ≠ 0)
+: 0 < s.supply (AtomicTok.toMint (AMMSet.exists_imp_dif h)) := by
+  induction t with
+  | empty accs _ => 
+    exfalso
+    simp [AMMSet.empty] at h
+
+  | dep0 s' _ d ih =>
+    apply @Decidable.byCases ((AtomicTok.toMint (AMMSet.exists_imp_dif h))=(AtomicTok.toMint d.hdif))
+    . intro eq; rw [eq]
+      simp [Deposit0.apply, State.supply]
+      rw [AccountSet.supply_addb_same (((s'.accs.subb d.a d.t0 d.r0).subb d.a d.t1 d.r1)) (AtomicTok.toMint d.hdif) d.a d.r0]
+      apply NNReal.neq_zero_imp_gt
+      exact NNReal.pos_imp_add_pos d.r0 _ (d.r0.coe_nnreal_pos)
+
+    . intro neq
+      simp [neq]
+      simp [AtomicTok.toMint_diff neq] at h
+      exact ih h
+  
+  | swap s' _ sw ih =>
+    rw [Swap.mintedSupply]
+    have h' := Swap.amm_in_apply h
+    exact ih h'
